pulse/lib/pulse/lib/Pulse.Lib.Tank.fst
@@ -1,0 +1,111 @@
+(*
+   Copyright 2025 Microsoft Research
+
+   Licensed under the Apache License, Version 2.0 (the "License");
+   you may not use this file except in compliance with the License.
+   You may obtain a copy of the License at
+
+       http://www.apache.org/licenses/LICENSE-2.0
+
+   Unless required by applicable law or agreed to in writing, software
+   distributed under the License is distributed on an "AS IS" BASIS,
+   WITHOUT WARRANTIES OR CONDITIONS OF ANY KIND, either express or implied.
+   See the License for the specific language governing permissions and
+   limitations under the License.
+*)
+module Pulse.Lib.Tank
+#lang-pulse
+open Pulse.Lib.Pervasives
+module MS = Pulse.Lib.PCM.MonoidShares
+module GPR = Pulse.Lib.GhostPCMReference
+
+let pcm_of (n:nat) = MS.pcm_of MS.nat_plus_cm n
+
+let tank (n:nat) = GPR.gref (pcm_of n)
+
+inline_for_extraction
+instance non_informative_tank (n:nat)
+  : Pulse.Lib.NonInformative.non_informative (tank n)
+  = { reveal = ((fun x -> x) <: Pulse.Lib.NonInformative.revealer (tank n)) }
+
+let owns #n ([@@@mkey] g : tank n) (i:nat)
+: timeless_slprop
+= GPR.pts_to #_ #(pcm_of n) g i
+
+ghost
+fn alloc (n:nat)
+  returns g : tank n
+  ensures  owns g n
+{
+  let g = GPR.alloc #_ #(pcm_of n) n;
+  fold (owns g n);
+  g
+}
+
+ghost
+fn extract_bound (#n:nat) (g:tank n) (#i:erased nat)
+requires
+  owns g i
+ensures
+  owns g i ** pure (i <= n)
+{
+  unfold owns;
+  let v = GPR.read_simple g; 
+  fold owns;
+}
+
+[@@allow_ambiguous]
+ghost
+fn gather (#n:nat) (g:tank n) (#i #j:erased nat)
+requires
+  owns g i **
+  owns g j
+ensures
+  owns g (i + j) **
+  pure (i <= n /\ j <= n /\ i + j <= n)
+{
+  extract_bound g #i;
+  extract_bound g #j;
+  unfold (owns g i);
+  unfold (owns g j);
+  GPR.gather g _ _;
+  fold owns;
+  extract_bound g;
+}
+
+ghost
+fn share (#n:nat) (g:tank n) (#u #v:nat)
+requires
+  owns g (u + v)
+ensures
+  owns g u **
+  owns g v
+{
+  open FStar.PCM;
+  unfold owns;
+  rewrite (GPR.pts_to g (u + v))
+       as (GPR.pts_to g (op (pcm_of n) u v));
+  GPR.share g u v;
+  fold (owns g u);
+  fold (owns g v)
+}
+
+ghost
+fn share_one (#n:nat) (g:tank n) (#u:nat { u > 0 })
+requires
+  owns g u
+returns k:erased nat
+ensures
+  owns g (u - 1) **
+  owns g 1 **
+  pure (k == u - 1)
+{
+  open FStar.PCM;
+  unfold owns;
+  rewrite (GPR.pts_to g u)
+       as (GPR.pts_to g (op (pcm_of n) (u - 1) 1));
+  GPR.share g (u-1) 1;
+  fold (owns g (u - 1));
+  fold (owns g 1);
+  (hide #nat (u - 1))
+}
